more cleanup and prove std_int_interprets_std_sig

manualReflectionScript.sml
@@ -31,27 +31,27 @@ val out_bool_def = Define`
 
 (* Alternatively: out_bool ^mem ^indin x = @b. x = in_bool mem indin b *)
 
-val set_ind_def = xDefine "set_ind"`
+val set_ind_def = Define`
   set_ind ^mem ^indin = @indset. is_in mem indset indin`
 
-val in_ind_def = xDefine "in_ind"`
+val in_ind_def = Define`
   in_ind ^mem ^indin i = indin i`
 
-val out_ind_def = xDefine "out_ind"`
+val out_ind_def = Define`
   out_ind ^mem ^indin x = @i. indin i = x`
 
 (* Alternatively: out_ind ^mem ^indin x = @i. x = in_ind mem indin i *)
 
-val set_fun_ind_bool_def = xDefine "set_fun_ind_bool"`
+val set_fun_ind_bool_def = Define`
   set_fun_ind_bool ^mem ^indin =
     Funspace (set_ind mem indin) (set_bool mem indin)`
 
-val in_fun_ind_bool = xDefine "in_fun_ind_bool"`
+val in_fun_ind_bool = Define`
   in_fun_ind_bool ^mem ^indin f =
     Abstract (set_ind mem indin) (set_bool mem indin) \x.
       in_bool mem indin (f (out_ind mem indin x))`
 
-val out_fun_ind_bool_def = xDefine "out_fun_ind_bool"`
+val out_fun_ind_bool_def = Define`
   out_fun_ind_bool ^mem ^indin x = \i.
     out_bool mem indin (apply mem x (in_bool mem indin i))`
 
@@ -60,13 +60,12 @@ val out_fun_ind_bool_def = xDefine "out_fun_ind_bool"`
  *)
 
 
-
 (* Simple signatures etc. *)
 
-val std_type_env_def = xDefine "std_type_env"`
+val std_type_env_def = Define`
   std_type_env = FUPDATE_LIST FEMPTY ["fun", 2; "bool", 0; "ind", 0]`
 
-val std_term_env_def = xDefine "std_term_env"`
+val std_term_env_def = Define`
   std_term_env = FUPDATE_LIST FEMPTY
                    [ "=", Fun (Tyvar"A") (Fun (Tyvar"A") Bool)
                    ; "S", Fun (Fun (Tyvar"A")
@@ -77,18 +76,21 @@ val std_term_env_def = xDefine "std_term_env"`
                    ; "I", Fun (Tyvar"A") (Tyvar"A")
                    ]`
 
-val std_sig_def = xDefine "std_sig"`
+val std_sig_def = Define`
   std_sig = (std_type_env, std_term_env)`;
 
 val std_sig_thm = store_thm("std_sig_thm", ``is_std_sig std_sig``, EVAL_TAC)
 
 
-val std_tyass_def = xDefine "std_tyass"`
-     std_tyass ^mem ^indin "bool" [] = boolset
-  /\ std_tyass ^mem ^indin "ind" [] = set_ind mem indin
-  /\ std_tyass ^mem ^indin "fun" [x;y] = Funspace x y`
+val std_tyass_def = Define`
+     std_tyass ^mem ^indin tyop args =
+     case (tyop,args) of
+     | ("bool",[]) => boolset
+     | ("fun",[x;y]) => Funspace x y
+     | ("ind",[]) => set_ind mem indin
+     | _ => ∅`
 
-val std_tmass_def = xDefine "std_tmass"`
+val std_tmass_def = Define`
      std_tmass ^mem ^indin "=" [x] =
        (Abstract x (Funspace x boolset) \i.
           Abstract x boolset \j.
@@ -104,29 +106,44 @@ val std_tmass_def = xDefine "std_tmass"`
        Abstract x x (\i. i)`
 
 val std_int_def = xDefine "std_int"`
-  std_int ^mem ^indin = 
+  std_int ^mem ^indin =
     (std_tyass mem indin, std_tmass mem indin)`
 
-
-(*
-load "manualReflectionTheory";
-open manualReflectionTheory;
-open holSyntaxTheory finite_mapTheory;
-
-g `!mem indin. OK ==> is_interpretation std_sig (std_int mem indin)`;
-e GEN_TAC;
-e GEN_TAC;
-e DISCH_TAC;
-e EVAL_TAC;
-
-e CONJ_TAC;
-e (REWRITE_TAC [FEVERY_DEF]);
-e EVAL_TAC;
-
-e (RW_TAC (srw_ss()) []);
-e (Cases_on `ls`);
-e EVAL_TAC;
- *)
-
+val std_int_interprets_std_sig = store_thm("std_int_interprets_std_sig",
+ ``∀mem indin. ^OK ⇒ is_interpretation std_sig (std_int mem indin)``,
+ simp[is_interpretation_def,std_int_def] >>
+ rpt gen_tac >> strip_tac >>
+ conj_asm1_tac >- (
+   rw[is_type_assignment_def,FEVERY_ALL_FLOOKUP] >>
+   fs[std_sig_def,std_type_env_def,flookup_fupdate_list] >>
+   BasicProvers.EVERY_CASE_TAC >> rw[std_tyass_def] >>
+   BasicProvers.EVERY_CASE_TAC >> fs[]
+   >- metis_tac[funspace_inhabited]
+   >- metis_tac[mem_boolset]
+   >- (
+     rw[set_ind_def] >>
+     SELECT_ELIM_TAC >>
+     conj_tac >- metis_tac[] >>
+     rw[is_in_def] >> fs[BIJ_IFF_INV] >>
+     metis_tac[] )) >>
+ `is_std_type_assignment (std_tyass mem indin)` by (
+   rw[std_tyass_def,is_std_type_assignment_def,FUN_EQ_THM] ) >>
+ rw[is_term_assignment_def,FEVERY_ALL_FLOOKUP] >>
+ fs[std_sig_def,std_term_env_def,flookup_fupdate_list] >>
+ BasicProvers.EVERY_CASE_TAC >> rw[std_tmass_def] >>
+ CONV_TAC(ONCE_DEPTH_CONV(fn tm => if can (match_term``STRING_SORT (tyvars X)``) tm then EVAL tm else NO_CONV tm)) >>
+ imp_res_tac typesem_Fun >> rw[std_tmass_def] >> rw[typesem_def] >>
+ rw[std_tyass_def] >>
+ match_mp_tac (UNDISCH abstract_in_funspace) >> rw[] >>
+ match_mp_tac (UNDISCH abstract_in_funspace) >> rw[] >>
+ rw[in_bool_def,boolean_in_boolset] >>
+ match_mp_tac (UNDISCH abstract_in_funspace) >> rw[] >>
+ match_mp_tac (UNDISCH apply_in_rng) >>
+ qexists_tac`(τ "B")` >>
+ conj_tac >- (
+   match_mp_tac (UNDISCH apply_in_rng) >>
+   metis_tac[] ) >>
+ match_mp_tac (UNDISCH apply_in_rng) >>
+ metis_tac[] )
 
 val _ = export_theory()
